src/ADTRefinement/GeneralBuildADTRefinements.v
@@ -8,9 +8,9 @@ Require Import Coq.Lists.List Coq.Arith.Arith
         Fiat.ADTNotation.BuildComputationalADT
         Fiat.ADTNotation.BuildADTReplaceMethods
         Fiat.ADTRefinement.Core
-        Fiat.ADTRefinement.GeneralRefinements.
-(*         Fiat.ADTRefinement.SetoidMorphisms *)
-(*         Fiat.ADTRefinement.BuildADTSetoidMorphisms. *)
+        Fiat.ADTRefinement.GeneralRefinements
+        Fiat.ADTRefinement.SetoidMorphisms
+        Fiat.ADTRefinement.BuildADTSetoidMorphisms.
 
 (* Notation-friendly versions of the honing tactics in GeneralRefinements. *)
 
